codeTest/correct_test_complex.v
@@ -1,0 +1,159 @@
+From dx.tests Require Import DxIntegers DxValues DxMemRegion DxState DxMonad DxInstructions.
+From Coq Require Import List Lia.
+From compcert Require Import Integers Values Clight Memory.
+Import ListNotations.
+Require Import ZArith.
+
+From bpf.proof Require Import Clightlogic MatchState CorrectRel CommonLemma interpreter.
+
+(**
+
+unsigned long long test_complex(unsigned long long dst64, int imm)
+{
+  unsigned long long res;
+  res = get_addl(dst64, (unsigned long long) imm);
+  return res;
+}
+
+
+Definition test_complex (dst64: val64_t) (imm: sint32_t): M val64_t :=
+  do res <- get_addl dst64 (Val.longofintu (sint32_to_vint imm));
+  returnM res.
+
+ *)
+
+Ltac build_app_aux T :=
+  match T with
+  | ?F ?X => let ty := type of X in
+             let r := build_app_aux F in
+             constr:((mk ty X) :: r)
+  | ?X    => constr:(@nil dpair)
+  end.                                    
+
+Ltac get_function T :=
+  match T with
+  | ?F ?X => get_function F
+  | ?X    => X
+  end.
+
+Ltac build_app T :=
+  let a := build_app_aux T in
+  let v := (eval simpl in (DList.of_list_dp (List.rev a))) in
+  let f := get_function T in
+  match type of v with
+  | DList.t _ ?L =>
+      change T with (app (f: arrow_type L _) v)
+  end.
+
+Ltac change_app_for_body :=
+  match goal with
+  | |- @correct_body _ _ ?F _ _ _ _ _ _ _ _
+    => build_app F
+  end.
+
+Ltac change_app_for_statement :=
+  match goal with
+  | |- @correct_statement _ _ ?F _ _ _ _ _ _ _ _
+    => build_app F
+  end.
+
+Ltac prove_incl :=
+  simpl; unfold incl; simpl; intuition congruence.
+
+Ltac prove_in_inv :=
+  simpl; intuition subst; discriminate.
+
+Ltac correct_forward :=
+  match goal with
+  | |- @correct_body _ _ (bindM ?F1 ?F2)  _
+                     (Ssequence
+                        (Ssequence
+                           (Scall _ _ _)
+                           (Sset ?V ?T))
+                        ?R)
+                     _ _ _ _ _ _  =>
+      eapply correct_statement_seq_body;
+      [ change_app_for_statement ;
+        let b := match T with
+                 | Ecast _ _ => constr:(true)
+                 | _         => constr:(false)
+                 end in
+        eapply correct_statement_call with (has_cast := b)
+      |]
+  | |- @correct_body _ _ (match  ?x with true => _ | false => _ end) _
+                     (Sifthenelse _ _ _)
+                     _ _ _ _ _ _  =>
+      eapply correct_statement_if_body; [prove_in_inv | destruct x ]
+  end.
+
+
+Section Test_complex.
+
+  (** The program contains our function of interest [fn] *)
+  Definition p : Clight.program := prog.
+
+  (* [Args,Res] provides the mapping between the Coq and the C types *)
+  (* Definition Args : list CompilableType := [stateCompilableType].*)
+  Definition args : list Type := [(val64_t:Type); (sint32_t:Type)].
+  Definition res : Type := (val64_t:Type).
+
+  (* [f] is a Coq Monadic function with the right type *)
+  Definition f : arrow_type args (M res) := test_complex.
+
+  Variable state_block: block. (**r a block storing all rbpf state information? *)
+
+  (* [fn] is the Cligth function which has the same behaviour as [f] *)
+  Definition fn: Clight.function := f_test_complex.
+
+  (* [match_arg] relates the Coq arguments and the C arguments *)
+  Definition match_arg_list : DList.t (fun x => x -> val -> stateM -> Memory.Mem.mem -> Prop) args :=
+    (DList.DCons (stateless val64_correct)                 
+       (DList.DCons (stateless sint32_correct)
+                    (DList.DNil _))).
+
+  (* [match_res] relates the Coq result and the C result *)
+  Definition match_res : res -> val -> stateM -> Memory.Mem.mem -> Prop := fun x v st m => val64_correct x v.
+
+  Instance correct_function3_test_complex : correct_function3 p args res f fn (nil) true match_arg_list match_res.
+  Proof.
+    correct_function_from_body.
+    correct_body.
+    (** how to use correct_* *)
+    unfold INV.
+    unfold f, test_complex.
+    repeat intro.
+    get_invariant_more _dst64.
+    get_invariant_more _imm.
+
+    unfold stateless, val64_correct in H1.
+    unfold stateless, sint32_correct in H3.
+    destruct H1 as (Hc_eq & (vl & Hvl_eq)).
+    subst v v0 c.
+
+    exists (Val.addl (Vlong vl) (Val.longofintu (Vint c0))), m, Events.E0.
+
+    repeat split; unfold step2.
+    -
+      apply Smallstep.plus_star.
+      repeat forward_plus.
+      (** TODO: adding Sreturn  more info by Ltac2 *)
+      eapply Smallstep.plus_one; eauto.
+      eapply step_return_1.
+      +
+        repeat econstructor; eauto.
+        Transparent Archi.ptr64.
+        unfold Cop.sem_binary_operation.
+        unfold Cop.sem_add, Cop.classify_add, Ctypes.typeconv; simpl.
+        unfold Cop.sem_binarith, Cop.sem_cast, Cop.classify_cast; simpl.
+        reflexivity.
+      + econstructor; eauto.
+      + reflexivity.
+    - simpl.
+      exists (Int64.add x0 x); reflexivity.
+    - simpl.
+      constructor.
+  Qed.
+
+End Get_addl.
+
+Existing Instance correct_function3_get_addl.
